NCML/Hilbert/Logics.lean
@@ -41,4 +41,22 @@ theorem LogicCKB.provable_N : (∼◇⊥) ∈ LogicCKB := by
   have h4 : (◇(□⊥) 🡒 ⊥) ∈ LogicCKB := axm (by grind);
   exact imp_trans h3 h4;
 
+section
+
+open ProvableBDHilbert
+
+variable {A B : BDFormula}
+
+/-- - [Pac24, Theorem 3] -/
+theorem LogicCKB.provable_DP : (◇(A ⋎ B) 🡒 ◇A ⋎ ◇B) ∈ LogicCKB := by
+  have h₁ : (A 🡒 □◇A) ∈ LogicCKB := axm (by grind);
+  have h₂ : (B 🡒 □◇B) ∈ LogicCKB := axm (by grind);
+  have h₃ : (◇(□(◇A ⋎ ◇B)) 🡒 ◇A ⋎ ◇B) ∈ LogicCKB := axm (by grind);
+  have h₄ : (A ⋎ B 🡒 □(◇A ⋎ ◇B)) ∈ LogicCKB :=
+    mp (mp orElim (imp_trans h₁ (mp kBox (nec orIntro₁))))
+      (imp_trans h₂ (mp kBox (nec orIntro₂)));
+  exact imp_trans (mp kDia (nec h₄)) h₃;
+
+end
+
 end
